Work towards toplevel theorems

theories/L6_PCPS/inline_correct.v
@@ -1,7 +1,7 @@
 Require Import Coq.ZArith.ZArith Coq.Lists.List Coq.Strings.String Coq.Sets.Ensembles Coq.Classes.Morphisms.
 Require Import compcert.lib.Maps compcert.lib.Coqlib.
 Require Import L6.cps L6.state L6.freshen L6.cps_util L6.cps_show L6.ctx L6.hoare L6.inline L6.rename L6.identifiers
-        L6.Ensembles_util L6.alpha_conv L6.functions L6.logical_relations L6.tactics L6.eval L6.map_util L6.inline_letapp.
+        L6.Ensembles_util L6.alpha_conv L6.functions L6.logical_relations L6.tactics L6.eval L6.map_util L6.inline_letapp L6.List_util.
 Require Import Common.compM Common.Pipeline_utils Libraries.CpdtTactics Libraries.maps_util.
 Require Import ExtLib.Structures.Monad.
 Require Import ExtLib.Structures.MonadState.
@@ -25,18 +25,18 @@ Section Inline_Eq.
          let s' := update_inFun _ IH f t xs e sig s in
          let f' := apply_r sig' f in
          xs' <- get_names_lst xs "" ;;
-         e' <- beta_contract _ IH d e (set_list (combine xs xs') sig') fm s' ;;
+         e' <- beta_contract _ IH d e (set_list (combine xs xs') sig') fm s' false ;;
          fds'' <- beta_contract_fds fds' s ;;
          ret (Fcons f' t xs' e' fds'')
        | Fnil => ret Fnil
        end).
   
-  Definition beta_contract' (d : nat) (e : exp) (sig : r_map) (fm:fun_map) (s:St) : inlineM exp :=
+  Definition beta_contract' (d : nat) (e : exp) (sig : r_map) (fm:fun_map) (s:St) (str_flag : bool) : inlineM exp :=
     match e with
     | Econstr x t ys e =>
       let ys' := apply_r_list sig ys in
       x' <- get_name x "" ;;
-      e' <- beta_contract _ IH d e (M.set x x' sig) fm s;;
+      e' <- beta_contract _ IH d e (M.set x x' sig) fm s str_flag ;;
       ret (Econstr x' t ys' e')
     | Ecase v cl =>
       let v' := apply_r sig v in
@@ -44,7 +44,7 @@ Section Inline_Eq.
                 match br with
                 | nil => ret ( nil)
                 | (t, e)::br' =>
-                  e' <- beta_contract _ IH d e sig fm s;;
+                  e' <- beta_contract _ IH d e sig fm s str_flag;;
                   br'' <- beta_list br';;
                   ret ((t, e')::br'')
                 end) cl;;
@@ -52,7 +52,7 @@ Section Inline_Eq.
     | Eproj x t n y e =>
       let y' := apply_r sig y in
       x' <- get_name x "" ;;
-      e' <- beta_contract _ IH d e (M.set x x' sig) fm s;;
+      e' <- beta_contract _ IH d e (M.set x x' sig) fm s str_flag;;
       ret (Eproj x' t n y' e')
     | Eletapp x f t ys ec =>
       let f' := apply_r sig f in
@@ -63,23 +63,23 @@ Section Inline_Eq.
          if (Nat.eqb (List.length xs) (List.length ys)) then 
            let sig' := set_list (combine xs ys') sig in
            x' <- get_name x "" ;;         
-           e' <- beta_contract _ IH d' e sig' (M.remove f fm) s' ;;
+           e' <- beta_contract _ IH d' e sig' (M.remove f fm) s' str_flag ;;
            match inline_letapp e' x', Nat.eqb (List.length xs) (List.length ys) with
            | Some (C, x'), true =>
-             ec' <- beta_contract _ IH d' ec (M.set x x' sig) fm s' ;;
+             ec' <- beta_contract _ IH d' ec (M.set x x' sig) fm s' str_flag ;;
              ret (C |[ ec' ]|)
            | _, _ =>
              x' <- get_name x "" ;;
-             ec' <- beta_contract _ IH d ec (M.set x x' sig) fm s' ;;
+             ec' <- beta_contract _ IH d ec (M.set x x' sig) fm s' str_flag ;;
              ret (Eletapp x' f' t ys' ec')
            end
          else              
            x' <- get_name x "" ;;
-           ec' <- beta_contract _ IH d ec (M.set x x' sig) fm s' ;;
+           ec' <- beta_contract _ IH d ec (M.set x x' sig) fm s' str_flag ;;
            ret (Eletapp x' f' t ys' ec')
        | _ =>
          x' <- get_name x "" ;;
-         ec' <- beta_contract _ IH d ec (M.set x x' sig) fm s' ;;
+         ec' <- beta_contract _ IH d ec (M.set x x' sig) fm s' str_flag ;;
          ret (Eletapp x' f' t ys' ec')
        end)
     | Efun fds e =>
@@ -89,7 +89,7 @@ Section Inline_Eq.
       names' <- get_names_lst names "" ;;
       let sig' := set_list (combine names names') sig in
       fds' <-  beta_contract_fundefs d sig sig' fm fds s2 ;;
-      e' <- beta_contract _ IH d e sig' fm' s1;;
+      e' <- beta_contract _ IH d e sig' fm' s1 str_flag ;;
       ret (Efun fds' e')
     | Eapp f t ys =>
       let f' := apply_r sig f in
@@ -97,16 +97,16 @@ Section Inline_Eq.
       let (s', inl) := update_App _ IH f' t ys' s in
       (match (inl, M.get f fm, d) with
        | (true, Some (ft, xs, e), S d') =>
-         if Nat.eqb (List.length xs) (List.length ys) then
+         if (Nat.eqb (List.length xs) (List.length ys) && (negb str_flag || straight_code e))%bool then
            let sig' := set_list (combine xs ys') sig  in
-           beta_contract _ IH d' e sig' (M.remove f fm)  s'
+           beta_contract _ IH d' e sig' (M.remove f fm)  s' str_flag
          else ret (Eapp f' t ys')
        | _ => ret (Eapp f' t ys')
        end)
     | Eprim x t ys e =>
       let ys' := apply_r_list sig ys in
       x' <- get_name x "" ;;
-      e' <- beta_contract _ IH d e (M.set x x' sig) fm s;;
+      e' <- beta_contract _ IH d e (M.set x x' sig) fm s str_flag;;
       ret (Eprim x' t ys' e')
     | Ehalt x =>
       let x' := apply_r sig x in
@@ -114,8 +114,8 @@ Section Inline_Eq.
     end.
   
   
-  Lemma beta_contract_eq (d : nat) (e : exp) (sig : r_map) (fm:fun_map) (s:St) : 
-    beta_contract _ IH d e sig fm s = beta_contract' d e sig fm s.
+  Lemma beta_contract_eq (d : nat) (e : exp) (sig : r_map) (fm:fun_map) (s:St) (str_flag : bool) : 
+    beta_contract _ IH d e sig fm s str_flag = beta_contract' d e sig fm s str_flag.
   Proof.
     destruct d; destruct e; try reflexivity.
   Qed.
@@ -994,7 +994,7 @@ Section Inline_correct.
              
    
   Lemma inline_correct_mut d : 
-    (forall e sig fm st S
+    (forall e sig fm st S str_flag 
             (Hun : unique_bindings e)
             (Hdis1 : Disjoint _ (bound_var e) (occurs_free e :|: occurs_free_fun_map fm))
             (Hdis1' : Disjoint _ (bound_var e :|: bound_var_fun_map fm) (image (apply_r sig) (occurs_free e :|: occurs_free_fun_map fm)))
@@ -1004,12 +1004,13 @@ Section Inline_correct.
             
             (Hfm : fun_map_vars fm S sig),
         {{ fun _ s => fresh S (next_var (fst s)) }}
-          beta_contract St IH d e sig fm st
+          beta_contract St IH d e sig fm st str_flag 
         {{ fun _ s e' s' =>
              fresh S (next_var (fst s')) /\ next_var (fst s) <= next_var (fst s') /\
              unique_bindings e' /\
              occurs_free e' \subset image (apply_r sig) (occurs_free e :|: occurs_free_fun_map fm) /\
              bound_var e' \subset (Range (next_var (fst s)) (next_var (fst s')))  /\ Ecase_shape sig e e' /\
+             (str_flag = true -> preserves_straight_code e e') /\ 
              (forall k rho1 rho2,
                  preord_env_P_inj cenv PG (occurs_free e) k (apply_r sig) rho1 rho2 ->
                  fun_map_inv d (occurs_free e) fm rho1 rho2 k sig ->
@@ -1074,8 +1075,8 @@ Section Inline_correct.
       + eapply Disjoint_Included_r. eapply bound_var_occurs_free_Econstr_Included. eassumption.
       + eapply fun_map_vars_set. eassumption.
       + intros e' w2. eapply return_triple.
-        intros _ st'. intros [Hf1 [Hf2 [Hf3 [Hf4 [Hun [Hsub [Hsub' Hsem]]]]]]].
-        split; [| split; [| split; [| split; [| split; [| split ]]]]].
+        intros _ st'. intros [Hf1 [Hf2 [Hf3 [Hf4 [Hun [Hsub [Hsub' [Hsh [Hstr Hsem]]]]]]]]].
+        split; [| split; [| split; [| split; [| split; [| split; [| split ]]]]]].
         * eapply fresh_monotonic;[| eassumption ]. sets.
         * zify; omega.
         * constructor; [| eassumption ].
@@ -1092,6 +1093,7 @@ Section Inline_correct.
           eapply Included_trans. eapply Singleton_Included. eassumption. eapply Range_Subset. reflexivity.
           zify; omega.
         * eauto.
+        * intros Hs. simpl in *. eauto. 
         * intros r1 r2 k Henv Hfm'. eapply preord_exp_constr_compat.
           now eauto. now eauto.
           eapply Forall2_preord_var_env_map. eassumption. normalize_occurs_free. now sets.          
@@ -1115,10 +1117,11 @@ Section Inline_correct.
         with (Q := fun r w l w' => fresh S (next_var (fst w)) /\ fresh S (next_var (fst w')) /\ l = [] /\ next_var (fst w) <= next_var (fst w')).
       now intros; eauto.
       intros xs w'. simpl. eapply return_triple. simpl; intros.  destructAll.
-      split; [| split; [| split; [| split; [| split; [| split ]]]]]; eauto.
+      split; [| split; [| split; [| split; [| split; [| split; [| split ]]]]]]; eauto.
       + constructor.
       + simpl. normalize_occurs_free. sets.
       + normalize_bound_var. sets.
+      + intros Heq Hs. inv Hs.
       + intros. eapply preord_exp_case_nil_compat. now eauto.
     - (* Ecase (_ :: _) *)
       simpl. setoid_rewrite assoc. eapply bind_triple.
@@ -1141,10 +1144,11 @@ Section Inline_correct.
         * eassumption.
       + intros e' w. simpl.
         eapply pre_curry_l. intros Hf. eapply pre_strenghtening.
-        { intros. destructAll.
-          eapply (conj H8 (conj H7 (conj H3 (conj H1 (conj H6 (conj H0 H)))))). }
+        { intros. destructAll. 
+          eapply (conj H9 (conj H8 (conj H7 (conj H3 (conj H1 (conj H6 (conj H0 H))))))). }
         
-        eapply pre_curry_l. intros Hrel. eapply pre_curry_l. intros Hcase. eapply pre_curry_l. intros Hfv. eapply pre_curry_l. intros Hun. 
+        eapply pre_curry_l. intros Hrel. eapply pre_curry_l. intros Hs. eapply pre_curry_l. intros Hcase.
+        eapply pre_curry_l. intros Hfv. eapply pre_curry_l. intros Hun. 
         setoid_rewrite st_eq_Ecase. eapply bind_triple.
         * setoid_rewrite beta_contract_eq in IHl. unfold beta_contract' in IHl.
           do 2 eapply frame_rule. eapply pre_transfer_r.
@@ -1166,7 +1170,7 @@ Section Inline_correct.
             eapply (conj H6 (conj H1 (conj H2' (conj H3 (conj H4' (conj H5' H7)))))). }
           eapply pre_curry_l. intros Hex. destructAll.
           eapply return_triple. intros. destructAll.
-          split; [| split; [| split; [| split; [| split; [| split ]]]]]; eauto.
+          split; [| split; [| split; [| split; [| split; [| split; [| split ]]]]]]; eauto.
           ++ zify; omega.
           ++ constructor. eassumption. eassumption.
              eapply Disjoint_Included. eassumption. eassumption. eapply Disjoint_Range. reflexivity.
@@ -1182,13 +1186,13 @@ Section Inline_correct.
              ** now eauto.
              ** now eauto.
              ** now eauto.
-             ** eapply H9. now constructor.
+             ** eapply H10. now constructor.
              ** intros. eapply Hrel.
                 --- eapply preord_env_P_inj_monotonic; [| eapply preord_env_P_inj_antimon; [ eassumption | ]].
                     omega. normalize_occurs_free. sets.
                 --- eapply fun_map_inv_antimon. eapply fun_map_inv_i_mon. eassumption. omega.
                     normalize_occurs_free. sets.
-             ** eapply H8.
+             ** eapply H9.
                 --- eapply preord_env_P_inj_monotonic; [| eapply preord_env_P_inj_antimon; [ eassumption | ]].
                     omega. normalize_occurs_free. sets.
                 --- eapply fun_map_inv_antimon. eassumption.
@@ -1218,8 +1222,8 @@ Section Inline_correct.
       + eapply Disjoint_Included_r. eapply bound_var_occurs_free_Eproj_Included. eassumption.
       + eapply fun_map_vars_set. eassumption.
       + intros e' w2. eapply return_triple.
-        intros _ st'. intros [Hf1 [Hf2 [Hf3 [Hf4 [Hun [Hsub [Hsub' Hsem]]]]]]].
-        split; [| split; [| split; [| split; [| split; [| split ]]]]].
+        intros _ st'. intros [Hf1 [Hf2 [Hf3 [Hf4 [Hun [Hsub [Hsub' [Hsh [Hstr Hsem]]]]]]]]].
+        split; [| split; [| split; [| split; [| split; [| split; [| split]]]]]].
         * eapply fresh_monotonic;[| eassumption ]. sets.
         * zify; omega.
         * constructor; [| eassumption ].
@@ -1235,6 +1239,7 @@ Section Inline_correct.
           eapply Included_trans. eapply Singleton_Included. eassumption. eapply Range_Subset. reflexivity.
           zify; omega.
         * eauto.
+        * intros Hs. simpl in *; eauto.
         * intros r1 r2 k Henv Hfm'. eapply preord_exp_proj_compat.
           now eauto. now eauto. eapply Henv. now constructor.
           intros. eapply Hsem. 
@@ -1279,8 +1284,8 @@ Section Inline_correct.
         - eapply Disjoint_Included_r. eapply bound_var_occurs_free_Eletapp_Included. eassumption.
         - eapply fun_map_vars_set. eassumption.
         - intros e' w2. eapply return_triple.
-          intros _ st'. intros [Hf1 [Hf2 [Hf3 [Hf4 [Hun [Hsub [Hsub' Hsem]]]]]]].
-          split; [| split; [| split; [| split; [| split; [| split ]]]]].
+          intros _ st'. intros [Hf1 [Hf2 [Hf3 [Hf4 [Hun [Hsub [Hsub' [Hsh [Hstr Hsem]]]]]]]]].
+          split; [| split; [| split; [| split; [| split; [| split; [| split ]]]]]].
           * eapply fresh_monotonic;[| eassumption ]. sets.
           * zify; omega.
           * constructor; [| eassumption ].
@@ -1298,6 +1303,7 @@ Section Inline_correct.
             eapply Included_trans. eapply Singleton_Included. eassumption. eapply Range_Subset. reflexivity.
             zify; omega.
           * simpl; eauto.
+          * intros Hs; eauto.
           * intros r1 r2 k Henv Hfm'. eapply preord_exp_letapp_compat.
             now eauto. now eauto. now eauto.
             eapply Henv. econstructor. now left.
@@ -1381,11 +1387,11 @@ Section Inline_correct.
                 assert (Hbv : bound_var ei \subset S \\ [set z]).
                 { eapply Included_trans. eassumption. intros y Hin. unfold Ensembles.In, Range in *. inv Hin.
                   eapply Hfz. eassumption. }
-                 
-                eapply (conj Hbv (conj H15 (conj H14 (conj H12 (conj H11 (conj H9 (conj H10 (conj H13 Hfr')))))))). }
-
-              eapply pre_curry_l. intros Hbv. 
-              eapply pre_curry_l. intros Hrel. eapply pre_curry_l. intros Hcase. eapply pre_curry_l. intros Hfv. eapply pre_curry_l. intros Hun.
+                
+                eapply (conj Hbv (conj H16 (conj H15 (conj H14 (conj H12 (conj H11 (conj H9 (conj H10 (conj H13 Hfr'))))))))). }
+              
+              eapply pre_curry_l. intros Hbv. eapply pre_curry_l. intros Hrel.
+              eapply pre_curry_l. intros Hstr. eapply pre_curry_l. intros Hcase. eapply pre_curry_l. intros Hfv. eapply pre_curry_l. intros Hun.
               
               assert (Hdisr : Disjoint var (S \\ [set z] \\ bound_var ei :|: (bound_var e :|: bound_var_fun_map fm)) [set r]).
               { edestruct inline_letapp_var_eq. eassumption.
@@ -1416,6 +1422,7 @@ Section Inline_correct.
                     eapply Disjoint_Included; [| | eapply Hdis1' ]; try now sets.
                     eapply Included_trans. eapply image_monotonic. eapply Included_Setminus_compat.
                     eapply occurs_free_fun_map_remove. reflexivity. now sets. }
+
               
               eapply bind_triple.
               + do 3 eapply frame_rule.
@@ -1444,7 +1451,7 @@ Section Inline_correct.
                     eapply Disjoint_Included_r. eapply image_apply_r_set.
                     eapply Union_Disjoint_r. now sets. now xsets. }
               + intros e' w''. eapply return_triple. intros _ w''' Hyp. destructAll.
-                split; [| split; [| split; [| split; [| split; [| split ]]]]].
+                split; [| split; [| split; [| split; [| split; [| split; [| split ]]]]]].
                 * eapply fresh_monotonic; [| eassumption ]. sets.
                 * zify; omega.
                 * eapply (proj1 (ub_app_ctx_f e')). split; [| split ]; [| eassumption |].
@@ -1460,8 +1467,8 @@ Section Inline_correct.
                 * eapply Included_trans. eapply occurs_fee_inline_letapp. eassumption.
                   assert (Hsub : occurs_free ei :|: (occurs_free e' \\ stemctx.bound_stem_ctx C) \subset
                                              occurs_free ei :|: (occurs_free e' \\ [set r])).
-                  { edestruct inline_letapp_var_eq_alt. eassumption. inv H19; subst. now sets.
-                    inv H19. now sets. rewrite Union_Setminus_Included with (s3 := [set r]); tci. sets.
+                  { edestruct inline_letapp_var_eq_alt. eassumption. inv H20; subst. now sets.
+                    inv H20. now sets. rewrite Union_Setminus_Included with (s3 := [set r]); tci. sets.
                     sets. }
                   eapply Included_trans. eassumption. eapply Union_Included.
                   -- eapply Included_trans. eassumption. eapply Included_trans.
@@ -1482,7 +1489,8 @@ Section Inline_correct.
                      eapply Singleton_Included. unfold Ensembles.In, Range in *. zify; omega.
                      eapply Included_trans. eassumption. eapply Range_Subset. zify; omega. zify; omega.
                   -- eapply Included_trans. eassumption. eapply Range_Subset. zify; omega. zify; omega.
-                * eauto.                     
+                * eauto.
+                * intros Heq Hs; eauto. eapply straight_code_ctx_app. eassumption. eapply H18; eauto.
                 * intros. eapply inline_letapp_correct_alt with (C' := Hole_c);
                             [ | | | | | | | | | | now eauto | eassumption ]. 
                   -- eassumption.
@@ -1490,9 +1498,9 @@ Section Inline_correct.
                   -- eassumption.
                   -- eassumption.
                   -- eauto.
-                  -- simpl. intros. edestruct H20 with (f0 := f). constructor. now left. eassumption. eassumption.
+                  -- simpl. intros. edestruct H21 with (f0 := f). constructor. now left. eassumption. eassumption.
                      destructAll. do 2 subst_exp. eapply Hrel.
-                     ++ edestruct preord_env_P_inj_get_list_l. now eapply H19. normalize_occurs_free. now sets.
+                     ++ edestruct preord_env_P_inj_get_list_l. now eapply H20. normalize_occurs_free. now sets.
                         eassumption. destructAll.                           
                         eapply preord_env_P_inj_set_lists_l'; try eassumption.
                         eapply preord_env_P_inj_monotonic; [| eassumption ]. omega.
@@ -1504,8 +1512,8 @@ Section Inline_correct.
                         ** eassumption.
                         ** eapply Union_Disjoint_r. now sets. rewrite Dom_map_remove. sets. 
                         ** rewrite Union_Setminus_Included. sets. tci. sets. 
-                  -- intros. edestruct H20 with (f0 := f). constructor. now left. eassumption. eassumption.
-                     destructAll. subst_exp. eapply H18.
+                  -- intros. edestruct H21 with (f0 := f). constructor. now left. eassumption. eassumption.
+                     destructAll. subst_exp. eapply H19.
                      ++ rewrite apply_r_set_f_eq. eassumption.
                      ++ eapply fun_map_inv_antimon.
                         2:{ eapply Included_trans. eapply Included_Union_Setminus with (s2 := [set x]); tci.
@@ -1520,9 +1528,9 @@ Section Inline_correct.
                            normalize_bound_var_ctx. normalize_sets. intros y Hin Hin'.
                            eapply bound_var_inline_letapp in Hin'; [| eassumption ]. eapply Hdis2.
                            constructor. 2:{ right. rewrite image_Union. right. eassumption. }
-                           inv Hin'. inv H29.
+                           inv Hin'. inv H30.
                            eapply Hfx. unfold Ensembles.In, Range in *. zify; omega.
-                           eapply H11 in H29. eapply Hfx. unfold Ensembles.In, Range in *. zify; omega.
+                           eapply H11 in H30. eapply Hfx. unfold Ensembles.In, Range in *. zify; omega.
                         ** eassumption.
                         ** intros Hc. eapply Hdis3. constructor. 2:{ eassumption. } now eauto.
                         ** intros Hc. eapply Hdis1. constructor. now constructor. now eauto.
@@ -1551,18 +1559,6 @@ Section Inline_correct.
       simpl. destruct (update_funDef St IH f2 sig st). 
       eapply bind_triple. eapply pre_transfer_r. now eapply get_names_lst_fresh. intros xs w. simpl.
       eapply pre_curry_l. intros Hf. eapply pre_curry_l. intros Hnd.  eapply pre_curry_l. intros Hlen.
-
-      (* assert (Hsame1 : bound_var_fundefs f2 \\ funname_in_fundefs f2 \\ name_in_fundefs f2 \subset bound_var (Efun f2 e) \\ funname_in_exp (Efun f2 e)). *)
-      (* { normalize_bound_var. simpl. rewrite !Setminus_Union_distr. eapply Included_Union_preserv_l. *)
-      (*   rewrite <- !Setminus_Union. eapply Included_Setminus; [| now sets ]. *)
-      (*   eapply Disjoint_Included_r. eapply funname_in_exp_subset. sets. }  *)
-
-      (* assert (Hsame2 : bound_var e \\ funname_in_exp e \subset bound_var (Efun f2 e) \\ funname_in_exp (Efun f2 e)). *)
-      (* { normalize_bound_var. simpl. rewrite !Setminus_Union_distr. eapply Included_Union_preserv_r. *)
-      (*   rewrite (Union_commut _ (funname_in_exp _)). rewrite <- Setminus_Union. eapply Included_Setminus; [| now sets ]. *)
-      (*   eapply Disjoint_Included_r. eapply Union_Included. eapply funname_in_fundefs_subset. *)
-      (*   eapply name_in_fundefs_bound_var_fundefs. sets. }  *)
-
       
       assert (Hfm' : fun_map_vars (add_fundefs f2 fm) (S \\ FromList xs) (set_list (combine (all_fun_name f2) xs) sig)).
       { eapply fun_map_vars_def_funs; (try now eauto).
@@ -1666,7 +1662,7 @@ Section Inline_correct.
 
 
       intros e' w''. eapply return_triple. intros _ w''' Hyp. destructAll.
-      split; [| split; [| split; [| split; [| split; [| split ]]]]].
+      split; [| split; [| split; [| split; [| split; [| split; [| split ]]]]]].
       * eapply fresh_monotonic; [| eassumption ]. sets.
       * zify; omega. 
       * constructor. eassumption. eassumption.
@@ -1674,7 +1670,7 @@ Section Inline_correct.
         eapply Union_Disjoint_r.
         -- eapply Disjoint_Included. eassumption. eassumption.
            eapply Disjoint_sym. eapply Disjoint_Range. reflexivity.
-        -- rewrite Same_set_all_fun_name. rewrite H13. rewrite Hseq.
+        -- rewrite Same_set_all_fun_name. rewrite H14. rewrite Hseq.
            eapply Disjoint_Included. eassumption. eassumption.
            eapply Disjoint_sym. eapply Disjoint_Range. zify; omega.
       * repeat normalize_occurs_free. eapply Union_Included.
@@ -1682,7 +1678,7 @@ Section Inline_correct.
            eapply occurs_free_fundefs_name_in_fundefs_Disjoint. reflexivity.
            eapply Setminus_Included_Included_Union. eapply Included_trans. eassumption.
            eapply Included_trans. eapply image_apply_r_set_list. now eauto.
-           rewrite (Same_set_all_fun_name fds'). rewrite H13.
+           rewrite (Same_set_all_fun_name fds'). rewrite H14.
            rewrite apply_r_list_eq; eauto. eapply Union_Included. now sets. 
            eapply Included_Union_preserv_l. rewrite <- Same_set_all_fun_name.
            rewrite Setminus_Union_distr. rewrite !image_Union. eapply Union_Included. now sets.
@@ -1690,7 +1686,7 @@ Section Inline_correct.
         -- eapply Included_trans. eapply Included_Setminus_compat. eassumption. reflexivity.
            eapply Setminus_Included_Included_Union. 
            eapply Included_trans. eapply image_apply_r_set_list. now eauto.
-           rewrite (Same_set_all_fun_name fds'). rewrite H13.
+           rewrite (Same_set_all_fun_name fds'). rewrite H14.
            rewrite apply_r_list_eq; eauto. eapply Union_Included. now sets.
            eapply Included_Union_preserv_l. rewrite <- Same_set_all_fun_name.
            rewrite Setminus_Union_distr. rewrite !image_Union. eapply Union_Included. now sets.
@@ -1702,10 +1698,11 @@ Section Inline_correct.
         -- eapply Included_trans.
            eapply Included_Union_Setminus with (s2 := name_in_fundefs fds'). now tci. eapply Union_Included.
            ++ eapply Included_trans. eassumption. eapply Range_Subset; zify; omega. 
-           ++ rewrite Same_set_all_fun_name. rewrite H13. rewrite Hseq.
+           ++ rewrite Same_set_all_fun_name. rewrite H14. rewrite Hseq.
               eapply Included_trans. eassumption. eapply Range_Subset; zify; omega. 
         -- eapply Included_trans. eassumption. eapply Range_Subset. zify; omega. reflexivity.
       * eauto.
+      * intros Hs; eauto.
       * intros k rho1 rho2 Henv Hfm''. eapply preord_exp_fun_compat.
         now eauto. now eauto.
         assert (Hrel : preord_env_P_inj cenv PG
@@ -1717,13 +1714,13 @@ Section Inline_correct.
           intros x HIn v Hgetx. destruct (Decidable_name_in_fundefs f2). destruct (Dec x).
           - rewrite def_funs_eq in Hgetx; [| now eauto ]. inv Hgetx. eexists. split.
             + rewrite def_funs_eq. reflexivity. eapply Same_set_all_fun_name. 
-              rewrite H13. rewrite FromList_apply_list. eapply In_image.
+              rewrite H14. rewrite FromList_apply_list. eapply In_image.
               rewrite <- Same_set_all_fun_name. eassumption.
             + rewrite preord_val_eq. intros vs1 vs2 j t1 ys1 e2 rho1' Hlen' Hfind Hset.
-              edestruct H14. eassumption. destructAll. 
+              edestruct H15. eassumption. destructAll. 
               edestruct set_lists_length2 with (xs2 := x0) (vs2 := vs2) (rho' := def_funs fds' fds' rho2 rho2). 
               now eauto. eassumption. now eauto. do 3 eexists. split. eassumption. split. now eauto. 
-              intros Hlt Hvs. eapply preord_exp_post_monotonic. eassumption. eapply H19. 
+              intros Hlt Hvs. eapply preord_exp_post_monotonic. eassumption. eapply H20. 
               * eapply preord_env_P_inj_set_lists_alt; [| eassumption | | | | | now eauto | now eauto ]. 
                 -- eapply preord_env_P_inj_antimon. eapply IHi. eassumption. omega.
                    normalize_occurs_free. sets.
@@ -1746,11 +1743,11 @@ Section Inline_correct.
                   - eapply unique_bindings_fun_in_fundefs. eapply find_def_correct. eassumption. eassumption. }
                 eapply fun_map_inv_antimon. eapply fun_map_inv_set_lists; [ | | | now eauto ].
                 eapply fun_map_inv_set_lists_r; [| | now eauto ]. 
-                -- rewrite <- Hseq. rewrite <- H13. eapply fun_map_inv_sig_extend_Disjoint.
+                -- rewrite <- Hseq. rewrite <- H14. eapply fun_map_inv_sig_extend_Disjoint.
                    eapply fun_map_inv_def_funs. eapply fun_map_inv_i_mon. eassumption. omega.
                    ++ eapply Disjoint_Included; [| | eapply Hdis1 ]. now sets. normalize_bound_var.
                       eapply Included_trans. eapply name_in_fundefs_bound_var_fundefs. now sets.
-                   ++ rewrite Same_set_all_fun_name, H13, Hseq. eapply Disjoint_Included ; [| | eapply Hdis2 ]. now sets. eassumption.
+                   ++ rewrite Same_set_all_fun_name, H14, Hseq. eapply Disjoint_Included ; [| | eapply Hdis2 ]. now sets. eassumption.
                    ++ eapply Disjoint_Included_l; [| eapply Hdis3 ]. normalize_bound_var.
                       eapply Included_trans. eapply name_in_fundefs_bound_var_fundefs. now sets.
                    ++ sets.
@@ -1772,22 +1769,22 @@ Section Inline_correct.
           - inv HIn. contradiction. rewrite def_funs_neq in Hgetx; [| eassumption ]. eapply Henv in Hgetx; [| eassumption ]. destructAll. 
             eexists. rewrite apply_r_set_list_f_eq. rewrite extend_lst_gso. rewrite def_funs_neq. 
             split; eauto. eapply preord_val_monotonic. eassumption. omega. 
-            + intros Hc. eapply Same_set_all_fun_name in Hc. rewrite H13 in Hc. 
+            + intros Hc. eapply Same_set_all_fun_name in Hc. rewrite H14 in Hc. 
               rewrite apply_r_list_eq in Hc; [| | now eauto ]. eapply Hdis2. constructor. 
               2:{ right. eapply In_image. eauto. } 
               eapply fresh_Range. 2:{ eapply Hsub. eassumption. } eassumption. eassumption.
             + rewrite <- Same_set_all_fun_name. intros Hc. eapply Hdis1. constructor. normalize_bound_var. left.
               now eapply name_in_fundefs_bound_var_fundefs. now eauto. }
-        eapply H9.
+        eapply H10.
         -- eapply preord_env_P_inj_antimon. eassumption. normalize_occurs_free.
            rewrite !Union_assoc. rewrite Union_Setminus_Included; sets. tci.
-        -- eapply fun_map_inv_antimon. rewrite <- Hseq. rewrite <- H13. eapply fun_map_inv_def_funs_add_fundefs.
-           eapply fun_map_inv_i_mon. eassumption. omega. rewrite H13, Hseq. eapply preord_env_P_inj_antimon.
+        -- eapply fun_map_inv_antimon. rewrite <- Hseq. rewrite <- H14. eapply fun_map_inv_def_funs_add_fundefs.
+           eapply fun_map_inv_i_mon. eassumption. omega. rewrite H14, Hseq. eapply preord_env_P_inj_antimon.
            eassumption. normalize_occurs_free. now sets. eassumption. normalize_occurs_free. sets.
            eapply Disjoint_Included_l. eapply name_in_fundefs_bound_var_fundefs.
            eapply Disjoint_Included; [| | eapply Hdis1 ]. now sets. normalize_bound_var. now sets.
 
-           rewrite Same_set_all_fun_name, H13, Hseq. eapply Disjoint_Included; [| | eapply Hdis2 ]. now sets. eassumption.
+           rewrite Same_set_all_fun_name, H14, Hseq. eapply Disjoint_Included; [| | eapply Hdis2 ]. now sets. eassumption.
            normalize_occurs_free. rewrite !Union_assoc. rewrite Union_Setminus_Included. now sets. tci. now sets.
     - (* Eapp *)
       simpl. destruct (update_App St IH (apply_r sig v) t (apply_r_list sig l) st) as [s b] eqn:Hup. 
@@ -1795,23 +1792,26 @@ Section Inline_correct.
         * destruct (fm ! v) as [[[ft xs] e] |] eqn:Heqf.
           destruct d.
           -- eapply return_triple.
-             intros. split; [| split; [| split; [| split; [| split; [| split ]]]]]; try eassumption.
+             intros. split; [| split; [| split; [| split; [| split; [| split; [| split ]]]]]]; try eassumption.
              ++ reflexivity.
              ++ constructor. 
              ++ repeat normalize_occurs_free. rewrite !image_Union, image_Singleton.
                 rewrite FromList_apply_list. sets.
              ++ normalize_bound_var. sets.
              ++ eauto.
+             ++ intros Heq Hs. eauto. 
              ++ intros. eapply preord_exp_app_compat.
                 now eauto. now eauto.
                 eapply H0. now constructor.
                 eapply Forall2_preord_var_env_map. eassumption.
                 now constructor.              
-          -- destruct (Datatypes.length xs =? Datatypes.length l)%nat eqn:Hbeq.
-             { symmetry in Hbeq. eapply beq_nat_eq in Hbeq.      
+          -- destruct ((Datatypes.length xs =?  Datatypes.length l)%nat &&
+                       (negb str_flag || straight_code e)) eqn:Hbeq.
+             { eapply andb_true_iff in Hbeq. inv Hbeq. symmetry in H. eapply beq_nat_eq in H.
+               eapply orb_true_iff in H0.
                edestruct Hfm. eassumption. destructAll. eapply post_weakening; [| eapply IHd ].
                ++ simpl. intros. destructAll.  
-                  split; [| split; [| split; [| split; [| split; [| split ]]]]]; try eassumption.
+                  split; [| split; [| split; [| split; [| split; [| split; [| split ]]]]]]; try eassumption.
                   ** eapply Included_trans. eassumption. 
                      eapply Included_trans. eapply image_apply_r_set_list.
                      unfold apply_r_list. rewrite list_length_map. eassumption.
@@ -1823,13 +1823,14 @@ Section Inline_correct.
                      eapply image_monotonic. eapply Included_trans. eapply Setminus_Included.
                      eapply occurs_free_fun_map_remove. 
                   ** eauto.
+                  ** intros Heq _. inv H0. simpl in *. congruence. eauto. eapply H16; eauto.
                   ** intros. eapply preord_exp_app_l.
                      --- eauto.
                      --- eauto.
-                     --- intros. assert (Hf := H16). assert (Heqf' := Heqf).
-                         edestruct H16; eauto. destructAll.
-                         do 2 subst_exp. eapply H14.
-                         +++ edestruct preord_env_P_inj_get_list_l. now eapply H15. normalize_occurs_free. now sets.
+                     --- intros. assert (Hf := H19). assert (Heqf' := Heqf).
+                         edestruct H19; eauto. destructAll.
+                         do 2 subst_exp. eapply H17.
+                         +++ edestruct preord_env_P_inj_get_list_l. now eapply H18. normalize_occurs_free. now sets.
                              eassumption. destructAll.                           
                              eapply preord_env_P_inj_set_lists_l'; try eassumption.
                          +++ eapply fun_map_inv_antimon. eapply fun_map_inv_set_lists; [ | | | eassumption ].
@@ -1842,7 +1843,7 @@ Section Inline_correct.
                              *** rewrite Union_Setminus_Included. sets. tci. sets.
                ++ omega.
                ++ eassumption.
-               ++ eapply Union_Disjoint_r. eapply Disjoint_Included; [| | eapply H1 ]; now sets.
+               ++ eapply Union_Disjoint_r. eapply Disjoint_Included; [| | eapply H3 ]; now sets.
                   sets. 
                ++ eapply Disjoint_Included_r. eapply image_apply_r_set_list.
                   unfold apply_r_list. rewrite list_length_map. eassumption.
@@ -1865,7 +1866,7 @@ Section Inline_correct.
                   eapply Included_trans; [| eapply bound_var_fun_map_get; eauto ]. now sets.
                ++ eapply Union_Disjoint_r.
                   eapply Union_Disjoint_r. now sets.
-                  clear H6. eapply Disjoint_Included_r. eapply bound_var_fun_map_remove. now sets.
+                  clear H8. eapply Disjoint_Included_r. eapply bound_var_fun_map_remove. now sets.
                   eapply Disjoint_Included_r. eapply image_apply_r_set_list.
                   unfold apply_r_list. rewrite list_length_map. eassumption.
                   eapply Disjoint_Included_r; [ | eapply Hdis2 ]. normalize_occurs_free.
@@ -1888,39 +1889,42 @@ Section Inline_correct.
                   eapply Disjoint_Included_r; [| eapply Hdis2 ]. normalize_occurs_free.
                   rewrite image_Union. rewrite FromList_apply_list. now sets. now sets. }
              { eapply return_triple. 
-               intros. split; [| split; [| split; [| split; [| split; [| split ]]]]]; try eassumption.
+               intros. split; [| split; [| split; [| split; [| split; [| split; [| split ]]]]]]; try eassumption.
                ++ reflexivity.
                ++ constructor.
                ++ simpl. repeat normalize_occurs_free. rewrite !image_Union, image_Singleton.
                   rewrite FromList_apply_list. sets.
                ++ normalize_bound_var. sets.
                ++ eauto.
+               ++ intros Heq Hs; eauto.
                ++ intros. eapply preord_exp_app_compat.
                   now eauto. now eauto.
                   eapply H0. now constructor.
                   eapply Forall2_preord_var_env_map. eassumption.
                   now constructor. }
           -- eapply return_triple.
-             intros. split; [| split; [| split; [| split; [| split; [| split ]]]]]; try eassumption.
+             intros. split; [| split; [| split; [| split; [| split; [| split; [| split ]]]]]]; try eassumption.
              ++ reflexivity.
              ++ constructor.
              ++ simpl. repeat normalize_occurs_free. rewrite !image_Union, image_Singleton.
                 rewrite FromList_apply_list. sets.
              ++ normalize_bound_var. sets.
              ++ eauto.
+             ++ intros Heq Hs; eauto.                                  
              ++ intros. eapply preord_exp_app_compat.
                 now eauto. now eauto.
                 eapply H0. now constructor.
                 eapply Forall2_preord_var_env_map. eassumption.
                 now constructor.
         *  eapply return_triple.
-           intros. split; [| split; [| split; [| split; [| split; [| split ]]]]]; try eassumption.
+           intros. split; [| split; [| split; [| split; [| split; [| split; [| split ]]]]]]; try eassumption.
            ++ reflexivity.
            ++ constructor.
            ++ simpl. repeat normalize_occurs_free. rewrite !image_Union, image_Singleton.
               rewrite FromList_apply_list. sets.
            ++ normalize_bound_var. sets.
-           ++ eauto.                              
+           ++ eauto.
+           ++ intros Heq Hs; eauto.
            ++ intros. eapply preord_exp_app_compat.
               now eauto. now eauto.
               eapply H0. now constructor.
@@ -1951,8 +1955,8 @@ Section Inline_correct.
       + eapply Disjoint_Included_r. eapply bound_var_occurs_free_Eprim_Included. eassumption.
       + eapply fun_map_vars_set. eassumption.
       + intros e' w2. eapply return_triple.
-        intros _ st'. intros [Hf1 [Hf2 [Hf3 [Hf4 [Hun [Hsub [Hsub' Hsem]]]]]]].
-        split; [| split; [| split; [| split; [| split; [| split ]]]]].
+        intros _ st'. intros [Hf1 [Hf2 [Hf3 [Hf4 [Hun [Hsub [Hsub' [Hsh [Hstr Hsem]]]]]]]]].
+        split; [| split; [| split; [| split; [| split; [| split; [| split ]]]]]].
         * eapply fresh_monotonic;[| eassumption ]. sets.
         * zify; omega.
         * constructor; [| eassumption ].
@@ -1969,17 +1973,19 @@ Section Inline_correct.
           eapply Included_trans. eapply Singleton_Included. eassumption. eapply Range_Subset. reflexivity.
           zify; omega.
         * eauto.
+        * intros Heq Hs; simpl in *; eapply Hstr; eauto. 
         * intros r1 r2 k Henv Hfm'. eapply preord_exp_prim_compat.
           now eauto.
           eapply Forall2_preord_var_env_map. eassumption. normalize_occurs_free. now sets.
     - (* Ehalt *)
       eapply return_triple.
-      intros. split; [| split; [| split; [| split; [| split; [| split ]]]]]; eauto.
+      intros. split; [| split; [| split; [| split; [| split; [| split; [| split ]]]]]]; eauto.
       + reflexivity.
       + constructor.
       + repeat normalize_occurs_free. rewrite image_Union, image_Singleton. sets.
       + normalize_bound_var. sets.
       + simpl; eauto.
+      + intros Heq Hs; eauto.
       + intros. eapply preord_exp_halt_compat. now eauto. now eauto.
         eapply H0. now constructor.
     - (* Fcons *)
@@ -2067,9 +2073,9 @@ Section Inline_correct.
         * intros Hc. eapply Included_Union_Setminus with (s2 := name_in_fundefs B') in Hc; [| tci ].
           inv Hc. 
           -- eapply Hnames2. constructor. 2:{ left. reflexivity. } left. 
-             eapply HSin. eapply H13 in H21. unfold Ensembles.In, Range in H21. zify; omega.
-          -- rewrite Same_set_all_fun_name in H21. rewrite H14 in H21. rewrite FromList_apply_list in H21.
-             inv Hnames1. eapply H24; eauto. eapply FromList_apply_list. eassumption.
+             eapply HSin. eapply H13 in H22. unfold Ensembles.In, Range in H22. zify; omega.
+          -- rewrite Same_set_all_fun_name in H22. rewrite H14 in H22. rewrite FromList_apply_list in H22.
+             inv Hnames1. eapply H25; eauto. eapply FromList_apply_list. eassumption.
              
         * eapply Disjoint_Included. eassumption. eassumption. eapply Disjoint_sym. eapply Disjoint_Range. reflexivity.
         * eapply Disjoint_Included_l. eapply Included_Union_Setminus with (s2 := name_in_fundefs B'); tci. eapply Union_Disjoint_l.
@@ -2109,12 +2115,12 @@ Section Inline_correct.
           eapply Included_trans. eassumption. eapply Range_Subset; zify; omega.
       + simpl. rewrite H14. reflexivity.
       + intros. destruct (cps.M.elt_eq f v); subst.
-        * inv H21. do 2 eexists. split; [| split; [| split; [| split ]]].
+        * inv H22. do 2 eexists. split; [| split; [| split; [| split ]]].
           -- simpl. rewrite peq_true. reflexivity.
           -- now eauto.
           -- eassumption.
           -- intros z HIn. eapply HSin. eapply Hxs in HIn. unfold Ensembles.In, Range in HIn. zify; omega.
-          -- intros. eapply H20.
+          -- intros. eapply H21.
              ++ rewrite apply_r_set_list_f_eq.
                 eapply preord_env_P_inj_antimon. eassumption. eapply Included_trans.
                 eapply occurs_free_in_fun with (B := (Fcons v ft xs0 e1 f5)). now left.
@@ -2124,12 +2130,12 @@ Section Inline_correct.
                 sets.
         * edestruct H15. eassumption. destructAll.
           do 2 eexists. split; [| split; [| split; [| split ]]].
-          -- simpl. rewrite peq_false. eassumption. intros Hc. inv Hnames1. eapply H29. rewrite <- Hc.
+          -- simpl. rewrite peq_false. eassumption. intros Hc. inv Hnames1. eapply H30. rewrite <- Hc.
              rewrite <- H14. eapply Same_set_all_fun_name. eapply find_def_name_in_fundefs. eassumption.
           -- now eauto.
           -- eassumption.
           -- eapply Included_trans. eassumption. sets.
-          -- intros. eapply H26; eauto.
+          -- intros. eapply H27; eauto.
              ++ eapply preord_env_P_inj_antimon. eassumption. normalize_occurs_free.
                 rewrite <- !Union_assoc.
                 rewrite <- Union_Included_Union_Setminus with (s1 := occurs_free_fundefs _) (s3 := [set v]).
@@ -2167,26 +2173,26 @@ Section Inline_correct.
     split; sets.
     intros x Hin. inv Hin. destructAll. rewrite M.gempty in H. inv H.
   Qed.
-
   
-  Lemma inline_correct_top d (e : exp) (st : St) (c:comp_data) rho1 rho2:
+
+  Lemma inline_correct_top d (e : exp) (st : St) (c:comp_data) :
     unique_bindings e ->
     Disjoint _ (bound_var e) (occurs_free e) ->
     (max_var e 1%positive) < (next_var c) ->
-    List_util.max_list (map fst (M.elements rho1)) 1%positive < next_var c ->
     exists e' c',
-      beta_contract_top St IH e d st c  = (Ret e', c') /\
+      beta_contract_top St IH e d st c true  = (Ret e', c') /\
       unique_bindings e' /\
       occurs_free e' \subset occurs_free e /\
-      (forall k,
+      preserves_straight_code e e' /\
+      (max_var e' 1%positive) < (next_var c') /\     
+      (forall k rho1 rho2,
           preord_env_P cenv PG (occurs_free e) k rho1 rho2 ->
           preord_exp cenv P1 PG k (e, rho1) (e', rho2)).
   Proof.
     intros. edestruct (inline_correct_mut d) as [He _].
     unfold beta_contract_top, triple in *.
     
-    specialize (He e (M.empty _) (M.empty _) st
-                   (fun x => Pos.max (max_var e 1%positive) (List_util.max_list (map fst (M.elements rho1)) 1%positive) < x) H).
+    specialize (He e (M.empty _) (M.empty _) st (fun x => max_var e 1%positive < x) true H).
 
     rewrite occurs_free_fun_map_empty, bound_var_fun_map_empty in *.
     repeat normalize_sets.
@@ -2197,13 +2203,13 @@ Section Inline_correct.
     { rewrite image_apply_r_empty. sets. } 
 
     
-    assert (Hdis1 : Disjoint var (fun x : var => Pos.max (max_var e 1) (List_util.max_list (map fst (M.elements rho1)) 1) < x)
+    assert (Hdis1 : Disjoint var (fun x : var => max_var e 1 < x)
                              (bound_var e :|: image (apply_r (M.empty var)) (occurs_free e))).
     { rewrite apply_r_empty_f_eq. rewrite image_id.  
-      constructor. intros x Hnin. inv Hnin. inv H4. 
-      eapply bound_var_leq_max_var with (y := 1%positive) in H5. unfold Ensembles.In in *. zify. omega.
-      eapply occurs_free_leq_max_var with (y := 1%positive) in H5. unfold Ensembles.In in *. zify. omega. }
-
+      constructor. intros x Hnin. inv Hnin. inv H3.
+      eapply bound_var_leq_max_var with (y := 1%positive) in H4. unfold Ensembles.In in *. zify. omega.
+      eapply occurs_free_leq_max_var with (y := 1%positive) in H4. unfold Ensembles.In in *. zify. omega. }
+    
 
     
     assert (Hdis2 : Disjoint var (bound_var e) (Dom_map (M.empty (fun_tag * list var * exp)))).
@@ -2213,11 +2219,11 @@ Section Inline_correct.
     { sets. }      
 
     assert (Hfinv : fun_map_vars (M.empty (fun_tag * list var * exp))
-                                 (fun x : var => Pos.max (max_var e 1) (List_util.max_list (map fst (M.elements rho1)) 1) < x)
+                                 (fun x : var => max_var e 1 < x)
                                  (M.empty var)).
-    { unfold fun_map_vars. intros. rewrite M.gempty in H3. inv H3. }
+    { unfold fun_map_vars. intros. rewrite M.gempty in H2. inv H2. }
     
-    assert (Hf : fresh (fun x : var => Pos.max (max_var e 1) (List_util.max_list (map fst (M.elements rho1)) 1) < x) (next_var (fst (c, tt)))).
+    assert (Hf : fresh (fun x : var => max_var e 1 < x) (next_var (fst (c, tt)))).
     { unfold fresh. intros. unfold Ensembles.In in *. simpl in *. zify; omega. }
 
     specialize (He Hdis Hdis1 Hdis2 Hdis3 Hfinv tt (c, tt) Hf).
@@ -2225,18 +2231,25 @@ Section Inline_correct.
     unfold runState, run_compM. simpl in *. 
     
     destruct (compM.runState
-                (beta_contract St IH d e (cps.M.empty var) (cps.M.empty (fun_tag * list var * exp)) st) tt (c, tt)) eqn:Heq.   
+                (beta_contract St IH d e (cps.M.empty var) (cps.M.empty (fun_tag * list var * exp)) st true) tt (c, tt)) eqn:Heq.   
     
     destruct e0. contradiction. destructAll.
     
-    destruct p. do 2 eexists. split; [| split; [| split ]].
+    destruct p. do 2 eexists. split; [| split; [| split; [| split; [| split ]]]].
     - reflexivity.
     - eassumption.
     - eapply Included_trans. eassumption. rewrite apply_r_empty_f_eq. rewrite image_id, occurs_free_fun_map_empty.
       sets.
+    - eapply H8; eauto.
+    - assert (Hin := max_var_subset e0). assert (Hin' := max_var_subset e).      
+      inv Hin.
+      + eapply H6 in H10. unfold Ensembles.In, Range in H10. simpl. inv H10. eassumption.
+      + eapply H5 in H10. rewrite occurs_free_fun_map_empty in H10. 
+        rewrite apply_r_empty_f_eq in H10. rewrite image_id in H10. repeat normalize_sets.
+        eapply occurs_free_leq_max_var in H10. eapply Pos.le_lt_trans. eassumption.
+        eapply H2. reflexivity.
     - intros. eapply H9; eauto. rewrite apply_r_empty_f_eq.
       intros x Hin. unfold id. now eauto.
-
       intro; intros. rewrite M.gempty in H12; inv H12.
   Qed. 
 
