theories/L6_PCPS/rel_comp.v
@@ -58,20 +58,6 @@ Definition wf_trivial {A} : A -> A -> Prop := fun _ _ => True.
 
 Definition preserves_fv (e1 e2 : exp) := occurs_free e2 \subset occurs_free e1.
 
-Fixpoint straight_code (e : exp) :=
-  match e with
-  | Econstr _ _ _ e
-  | Eprim _ _ _ e
-  | Eproj _ _ _ _ e
-  | Eletapp _ _ _ _ e 
-  | Efun _ e => straight_code e    
-  | Ecase _ _ => false 
-  | Eapp _ _ _ => true
-  | Ehalt _ => true
-  end.
-
-Definition preserves_straight_code (e1 e2 : exp) := straight_code e1 = true -> straight_code e2 = true.
-
 
 Section RelComp.
 
@@ -385,32 +371,7 @@ Section Linking.
     | None => None
     end.
 
-  
-  Lemma inline_straight_code_l (e : exp) x :
-    straight_code e = true ->
-    exists C x', inline_letapp e x = Some (C, x').
-  Proof.
-    intros.
-    induction e; simpl in *;
-      try (eapply IHe in H; destructAll; do 2 eexists; rewrite H; reflexivity).
-    - inv H.
-    - do 2 eexists. reflexivity.
-    - do 2 eexists. reflexivity.
-  Qed.
-
-  Lemma inline_straight_code_r (e : exp) x C x' :
-    inline_letapp e x = Some (C, x') ->
-    straight_code e = true.
-  Proof.
-    revert C x'.
-    induction e; intros C x' Hin; simpl in *;
-      try (match goal with
-           | [ _ : context[inline_letapp ?E ?X] |- _ ] => 
-             destruct (inline_letapp E X) as [[C' w] | ] eqn:Hin'; inv Hin
-           end); (try now inv Hin); try (now eauto).
-  Qed.
-
-  
+    
   Lemma link_straight_code_r x (e1 e2 e : exp) :
     link x e1 e2 = Some e ->
     straight_code e1 = true.
